Exercises for session 7, now solvable!

exercises/7/ex7.v
@@ -8,35 +8,62 @@ Load "ex6.v".
 
 Definition halts (t:tm) : Prop :=  exists t', t ⇒* t' /\ value t'.
 
-(* Exercise 1: Define R such that these properties hold:
+(* The logical relation we will use.
    Check Chapter 12 of Types and Programming Languages (Pierce)
 *)
-Definition R (T:ty) (t:tm) : Prop. Admitted.
+Fixpoint R (T:ty) (t:tm) : Prop :=
+    halts t /\ empty ⊢ t ∈ T /\
+    match T with
+      TBool         => True
+    | TArrow T1 T2  => forall u, R T1 u -> R T2 (tapp t u)
+    end.
 
 Lemma R_halts : forall {T} {t}, R T t -> halts t.
-Admitted.
+  intros.
+  induction T.
+  all: simpl in H; tauto.
+Defined.
 
 Lemma R_typable_empty : forall {T} {t}, R T t -> has_type empty t T.
+  intros.
+  induction T.
+  all: simpl in H; tauto.
+Defined.
+
+(* Exercise 1 (warm up): Show that the reduction relation is deterministic.
+   This is a very strong property; one may want to do the proof with a non-deterministic
+   reduction relation. *)
+Lemma red_deterministic : forall t a b  (r : t ⇒ a) (s :  t ⇒ b), a = b.
 Admitted.
 
+(* Exercise 2: Show that R is preserved by the reduction relation, back and forth: *)
 Lemma step_preserves_R : forall T t t', (t ⇒ t') -> R T t -> R T t'.
 Admitted.
 
-Lemma multistep_preserves_R : forall T t t', (t ⇒* t') -> R T t -> R T t'.
+Lemma step_preserves_R' : forall T t t', empty ⊢ t ∈ T ->  (t ⇒ t') -> R T t' -> R T t.
 Admitted.
 
-(* Exercise 2: Prove that R holds for well-typed, closed terms *)
-Lemma subst_R : forall Γ t T γ,
-    has_types empty γ Γ ->
-    has_type Γ t T ->
-    R T (t.[γ]).
+(* Exercise 3: *)
+
+(* We define the analogous of `R` for substitutions: *)
+Definition Rsubst Γ σ : Prop := has_types empty σ Γ /\ forall x T, Γ x = Some T -> R T (σ x).
+
+(* Show that R holds for all closed terms. 
+   For the induction to work, we need to consider a stronger property:  *)
+Lemma subst_R : forall Γ t T σ,
+    Rsubst Γ σ ->
+    Γ ⊢ t ∈ T ->
+    R T (t.[σ]).
 Admitted.
 
-(* Exercise 3: Using R_halts and subst_R, prove that the STλC is
-   strongly normalizing. 
-   You can do this even before doing Exercises 1 and 2.
+(* Then, proving closed_R is easy. *)
+Lemma closed_R : forall t T,  empty ⊢ t ∈ T -> R T t.
+Admitted.
+
+(* Exercise 4: Prove that the STλC is strongly normalizing.
+   You can do this exercise even before doing any of the earlier exercises.
  *)
 Lemma strong_normalization (t : tm) (T : ty) : empty ⊢ t ∈ T -> halts t.
 Admitted.
 
-(* BONUS: Do the exercise for the calculus extended with sums. *)
+(* BONUS: Extend the logical relation and the rest of the proof to work with sum types. *)
